FallDecoupled.v
@@ -2,6 +2,7 @@ Require Import FlowEquivalence.
 Require Import List.
 Import ListNotations.
 Open Scope list_scope.
+Require Import Monad.
 
 
 
@@ -13,6 +14,7 @@ Existing Instance latch_eq_dec.
 
 Require Import Coq.Logic.FunctionalExtensionality.
 Require Import Coq.Program.Equality.
+Require Import Omega. 
 
 
 Section FallDecoupled.
@@ -42,7 +44,6 @@ Section FallDecoupled.
                                               fd_place (Fall (Even E)) (Rise (Odd O))
   .
 
-  Require Import Monad.
 
   Definition fall_decoupled 
            : marked_graph (event even odd) :=
@@ -138,182 +139,350 @@ Ltac get_enabled_constraints :=
   end; specialize_enabled_constraints.
 
 
+Section loop_lemmas.
 
-Lemma odd_loop : forall t m,
-    {fall_decoupled}⊢ t ↓ m ->
-    forall O, m _ _ (Odd_rise O) + m _ _ (Odd_fall O) = 1.
-Admitted.
+  Variable t : trace even odd.
+  Variable m : marking fall_decoupled.
 
+  Hypothesis fd_t_m : {fall_decoupled}⊢ t ↓ m.
 
-Require Import Omega. 
-
-Lemma num_events_odd_rise_fall : forall t m,
-    {fall_decoupled}⊢ t ↓ m ->
-    forall O,
-    (m _ _ (Odd_fall O) = 1 -> num_events (Rise (Odd O)) t = 1 + num_events (Fall (Odd O)) t) /\
-    (m _ _ (Odd_rise O) = 1 -> num_events (Rise (Odd O)) t = num_events (Fall (Odd O)) t).
-Proof.
-Print mg_reachable.
-  intros t m Hm; induction Hm as [ | e' m m' t' Hm Hm'];
-    intros O op v Hv.
-  * split; intros Hinit; simpl in *; auto; find_contradiction.
-  * simpl in *.
-    split; intros Hinit; simpl in *; auto.
-    + repeat compare_next; auto.
-      { get_enabled_constraints.
-        unfold fire in *.
-        reduce_eqb.
-
-        inversion Hv; subst; simpl in *; reduce_eqb; find_contradiction.
-        assert (Hasync : ⟨c,init_st,P_FD⟩⊢ t' ↓ Odd O ↦{Transparent} next_state c st (Odd O)).
-        { econstructor; auto.
-          { (* if (Fall l) is enabled in m~t, then l is transparent in t *)
-            admit. }
-          { intros l' Hneighbor. specialize (H3 l' Hneighbor).
-            inversion Hneighbor; subst.
-            simpl in H3.
-          
-        }
-
-
-
-        contradict Hinit. 
-        omega.
-        simpl in *.
-
-  
-
-Lemma num_events_rise_fall : forall t l op v,
-    ⟨ c , init_st , P_FD ⟩⊢ t ↓ l ↦{ op } v ->
-    forall m,
-    {fall_decoupled}⊢ t ↓ m ->
-    (op = Opaque -> num_events (Fall l) t =
-                      match l with
-                      | Odd o => num_events (Rise (Odd o)) t
-                      | Even e => 1 + num_events (Rise (Even e)) t
-                      end)
-    /\
-    (op = Transparent -> num_events (Rise l) t = 
-                           match l with
-                           | Odd o => 1 + num_events (Fall (Odd o)) t
-                           | Even e => num_events (Fall (Even e)) t
-                           end).
-Proof.
-  induction t as [ | e t]; intros l op v Hv m Hm.
-  * split; intros Hop; subst; 
-    destruct l as [O | E];
-    simpl; auto;
-    inversion Hv;
-    inversion Hm;
-    subst;
-    find_contradiction.
-
-  * simpl in *.
-    repeat compare_next; auto.
-    + (* e = l- *)
-      inversion Hm; subst.
-      split; intros Hop; subst.
-      { inversion Hv; subst; find_contradiction.
-        assert (Hasync : ⟨c,init_st,P_FD⟩⊢ t ↓ l ↦{Transparent} next_state c st l).
-        { econstructor; auto.
-          (* if (Fall l) is enabled in m~t, then l is transparent in t *)
-          admit.
-        }
-        specialize (IHt _ _ _ Hasync _ H4).
-        destruct IHt as [IHt1 IHt2].
-        specialize (IHt2 eq_refl).
-        destruct l as [O | E]; reduce_eqb; auto.
-      }
-
-      { inversion Hv; subst; find_contradiction.
-        destruct l; reduce_eqb.
-        
-
-        assert (Hasync : ⟨c,init_st,P_FD⟩⊢ t ↓ l ↦{Transparent} next_state c st l).
-        { econstructor; auto.
-          (* if (Fall l) is enabled in m~t, then l is transparent in t *)
-          admit.
-        }
-
-        rewrite IHt2.
-    }
-        
-    
-
-    split; intros Hop; subst;
-    simpl;
-    auto;
-    inversion Hm; subst.
-    inversion Hv; subst;
-    find_contradiction;
-    try match goal with
-    | [ IH : forall l op v, ⟨c, init_st, P_FD⟩⊢ ?t ↓ l ↦{ op } v ->
-             forall m, {fall_decoupled}⊢ ?t ↓ m ->
-             _ /\ _
-      , H : ⟨c,init_st, P_FD⟩⊢ ?t ↓ _ ↦{_} _
-      , H' : {fall_decoupled}⊢ ?t ↓ _
-      |- _ ] =>
-        specialize (IH _ _ _ H _ H');
-        destruct IH as [IH1 IH2]
-    end.
-
-  * simpl in *. repeat compare_next; auto.
-  * simpl in *. repeat compare_next.
-    get_enabled_constraints.
-    specialize (IHt _ _ _ Hasync _ H4).
-    destruct IHt as [IH1 IH2].
-    rewrite IH2; auto.
-  * simpl in *. repeat compare_next; auto.
+  Lemma odd_loop : forall O, m _ _ (Odd_rise O) + m _ _ (Odd_fall O) = 1.
+  Proof.
+    intros O.
+    induction fd_t_m; auto.
+    subst; simpl; unfold fire.
+    repeat compare_next.
     { get_enabled_constraints. 
-    assert (Hasync : ⟨c,init_st,P_FD⟩⊢ t ↓ Odd O ↦{Transparent} next_state c st l).
-    { econstructor; auto.
-      (* if (Fall l) is enabled in m~t, then l is transparent in t *)
-      admit.
+      rewrite <- IHm0 at 3; auto.
+      omega.
     }
-      
-
-
-
-
-
-
-specialize (IHt (Odd O) _ _ H6 _ H4).
-      destruct IHt as [IH1 IH2].
-      auto.
+    { get_enabled_constraints. 
+      rewrite <- IHm0 at 3; auto.
+      omega.
     }
-  * simpl in *. repeat compare_next.
-    { 
-      , 
-specialize (IHt (Odd O) _ _ H6 _ H4).
-      destruct IHt as [IH1 IH2].
-      auto.
+    { apply IHm0; auto. }
+  Qed.
+
+
+  Lemma even_loop : forall E, m _ _ (Even_rise E) + m _ _ (Even_fall E) = 1.
+  Proof.
+    intros E. induction fd_t_m; auto.
+    subst; simpl; unfold fire.
+    repeat compare_next.
+    { get_enabled_constraints. etransitivity; [ | apply IHm0; auto]. omega. }
+    { get_enabled_constraints. etransitivity; [ | apply IHm0; auto]. omega. } 
+    { apply IHm0; auto. }
+  Qed.
+
+  Lemma even_odd_loop : forall E O (Hin : In (E,O) (even_odd_neighbors c)),
+        m _ _ (Even_rise_odd_rise E O Hin)
+      + m _ _ (Odd_fall O)
+      + m _ _ (Odd_fall_even_rise E O Hin)
+      = 1.
+  Proof.
+    intros E O  Hin.
+    induction fd_t_m; auto.
+    subst. unfold fire.
+    repeat compare_next.
+    { get_enabled_constraints.
+      etransitivity; [ | apply IHm0; auto].
+      omega.
     }
-    
+    { get_enabled_constraints.
+      etransitivity; [ | apply IHm0; auto].
+      omega.
+    }
+    { get_enabled_constraints.
+      etransitivity; [ | apply IHm0; auto].
+      omega.
+    }
+    { apply IHm0; auto. }
+  Qed.
 
-  intros t l op v Hasync.
-  induction Hasync; intros m Hm; split; intros Hop; subst; find_contradiction.
-  * destruct l; auto. find_contradiction.
-  * destructl 
+  Lemma odd_even_loop : forall O E (Hin : In (O,E) (odd_even_neighbors c)),
+        m _ _ (Odd_rise_even_rise O E Hin)
+      + m _ _ (Even_fall E)
+      + m _ _ (Even_fall_odd_rise O E Hin)
+      = 1.
+  Proof.
+    intros O E Hin.
+    induction fd_t_m; auto.
+    subst. unfold fire.
+    repeat compare_next.
+    { get_enabled_constraints.
+      etransitivity; [ | apply IHm0; auto].
+      omega.
+    }
+    { get_enabled_constraints.
+      etransitivity; [ | apply IHm0; auto].
+      omega.
+    }
+    { get_enabled_constraints.
+      etransitivity; [ | apply IHm0; auto].
+      omega.
+    }
+    { apply IHm0; auto. }
+  Qed.
 
-    inversion Hv; subst; simpl in *;
-    repeat compare_next; eauto;
-    destruct l as [O | E]; repeat compare_next; try (erewrite IHt; eauto; fail).
-    { erewrite IHt
-    
-Admitted.
+
+End loop_lemmas.
+
+Section fd_lemmas.
+
+  Variable t : trace even odd.
+  Variable m : marking fall_decoupled.
+
+  Hypothesis fd_t_m : {fall_decoupled}⊢ t ↓ m.
+
+  Lemma marking_odd_fall : forall O,
+    m _ _ (Odd_fall O) = match transparent t P_FD (Odd O) with
+                         | Opaque => 0
+                         | Transparent => 1
+                         end.
+  Proof.
+    induction fd_t_m; intros O; auto.
+    simpl.
+    set (loop := odd_loop t' m m0 O).
+    subst. unfold fire. 
+    repeat compare_next.
+    { get_enabled_constraints. omega. }
+    { get_enabled_constraints. omega. }
+    { rewrite IHm0; auto. }
+  Qed.
 
 
-Lemma num_events_odd_opaque : forall t  m O op v,
-    ⟨ c , init_st , P_FD ⟩⊢ t ↓ Odd O ↦{ Opaque } v ->
-    {fall_decoupled}⊢ t ↓ m ->
+  Lemma marking_odd_rise : forall O,
+    m _ _ (Odd_rise O) = match transparent t P_FD (Odd O) with
+                         | Opaque => 1
+                         | Transparent => 0
+                         end.
+  Proof.
+    induction fd_t_m; intros O; auto.
+    simpl.
+    set (loop := odd_loop t' m m0 O).
+    subst. unfold fire. 
+    repeat compare_next.
+    { get_enabled_constraints. omega. }
+    { get_enabled_constraints. omega. }
+    { rewrite IHm0; auto. }
+  Qed.
+
+  Lemma marking_even_fall : forall E,
+    m _ _ (Even_fall E) = match transparent t P_FD (Even E) with
+                         | Opaque => 0
+                         | Transparent => 1
+                         end.
+  Proof.
+    induction fd_t_m; intros E; auto.
+    simpl.
+    set (loop := even_loop t' m m0 E).
+    subst. unfold fire. 
+    repeat compare_next.
+    { get_enabled_constraints. omega. }
+    { get_enabled_constraints. omega. }
+    { rewrite IHm0; auto. }
+  Qed.
+
+  Lemma marking_even_rise : forall E,
+    m _ _ (Even_rise E) = match transparent t P_FD (Even E) with
+                         | Opaque => 1
+                         | Transparent => 0
+                         end.
+  Proof.
+    induction fd_t_m; intros E; auto.
+    simpl.
+    set (loop := even_loop t' m m0 E).
+    subst. unfold fire. 
+    repeat compare_next.
+    { get_enabled_constraints. omega. }
+    { get_enabled_constraints. omega. }
+    { rewrite IHm0; auto. }
+  Qed.
+
+  Lemma odd_num_events : forall O,
+    ( m _ _ (Odd_rise O) > 0 ->
+      num_events (Rise (Odd O)) t = num_events (Fall (Odd O)) t)
+    /\
+    ( m _ _ (Odd_fall O) > 0 ->
+      num_events (Rise (Odd O)) t = 1 + num_events (Fall (Odd O)) t).
+  Proof.
+    induction fd_t_m; intros O; split; intros Hrise; auto.
+    { contradict Hrise. simpl. inversion 1. }
+    { simpl in *.
+      set (loop := odd_loop t' m m0 O).
+      specialize (IHm0 m0 O).
+      destruct IHm0 as [IH1 IH2].
+      repeat compare_next; try unfold fire in Hrise; reduce_eqb.
+      { contradict Hrise. omega. }
+      { apply IH2; auto. }
+      { apply IH1; auto. }
+    }
+    { simpl in *.
+      set (loop := odd_loop t' m m0 O).
+      specialize (IHm0 m0 O).
+      destruct IHm0 as [IH1 IH2].
+      repeat compare_next; try unfold fire in Hrise; reduce_eqb.
+      { rewrite IH1; auto. }
+      { contradict Hrise. omega. }
+      { apply IH2; auto. }
+    }
+  Qed.
+
+  Lemma odd_rise_num_events : forall O,
+    m _ _ (Odd_rise O) > 0 ->
     num_events (Rise (Odd O)) t = num_events (Fall (Odd O)) t.
+  Proof.
+    intros O HO.
+    destruct (odd_num_events O) as [H _].
+    auto.      
+  Qed.
 
-Lemma num_events_even_opaque : forall t m E v,
-    ⟨ c , init_st , P_FD ⟩⊢ t ↓ Even E ↦{ Opaque } v ->
-    {fall_decoupled}⊢ t ↓ m ->
+  Lemma odd_fall_num_events : forall O,
+    m _ _ (Odd_fall O) > 0 ->
+    num_events (Rise (Odd O)) t = 1 + num_events (Fall (Odd O)) t.
+    intros O HO.
+    destruct (odd_num_events O) as [_ H].
+    auto.      
+  Qed.
+
+  Lemma even_num_events : forall E,
+    ( m _ _ (Even_rise E) > 0 ->
+      num_events (Fall (Even E)) t = 1 + num_events (Rise (Even E)) t)
+    /\
+    ( m _ _ (Even_fall E) > 0 ->
+      num_events (Fall (Even E)) t = num_events (Rise (Even E)) t).
+  Proof.
+    induction fd_t_m; intros E; split; intros Hrise; auto.
+    { contradict Hrise. simpl. inversion 1. }
+    { simpl in *.
+      set (loop := even_loop t' m m0 E).
+      specialize (IHm0 m0 E).
+      destruct IHm0 as [IH1 IH2].
+      repeat compare_next; try unfold fire in Hrise; reduce_eqb.
+      { rewrite IH2; auto. }
+      { contradict Hrise. omega. }
+      { rewrite IH1; auto. }
+    }
+    { simpl in *.
+      set (loop := even_loop t' m m0 E).
+      specialize (IHm0 m0 E).
+      destruct IHm0 as [IH1 IH2].
+      repeat compare_next; try unfold fire in Hrise; reduce_eqb.
+      { contradict Hrise. omega. }
+      { rewrite IH1; auto. }
+      { apply IH2; auto. }
+    }
+  Qed.
+
+
+  Lemma even_rise_num_events : forall E,
+    m _ _ (Even_rise E) > 0 ->
     num_events (Fall (Even E)) t = 1 + num_events (Rise (Even E)) t.
-Admitted. 
+  Proof.
+    intros E HE.
+    destruct (even_num_events E) as [H H'].
+    auto.      
+  Qed.
 
+  Lemma even_fall_num_events : forall E,
+    m _ _ (Even_fall E) > 0 ->
+    num_events (Fall (Even E)) t = num_events (Rise (Even E)) t.
+  Proof.
+    intros E HE.
+    destruct (even_num_events E) as [H H'].
+    auto.      
+  Qed.
+
+  Section even_odd.
+    Variable E : even.
+    Variable O : odd.
+    Hypothesis Hin : In (E,O) (even_odd_neighbors c).
+    
+    Lemma even_odd_num_events : 
+       (m _ _ (Odd_fall O) > 0 ->
+        num_events (Rise (Odd O)) t = 1 + num_events (Rise (Even E)) t)
+    /\ (m _ _ (Odd_fall_even_rise E O Hin) > 0 ->
+        num_events (Rise (Odd O)) t = 1 + num_events (Rise (Even E)) t)
+    /\ (m _ _ (Even_rise_odd_rise E O Hin) > 0 ->
+        num_events (Rise (Odd O)) t = num_events (Rise (Even E)) t).
+    Proof.
+      induction fd_t_m; repeat split; intros Hgt; simpl in *; auto; find_contradiction.
+      { set (Hloop := even_odd_loop t' m m0 E O Hin).
+        destruct (IHm0 m0) as [IH1 [IH2 IH3]].
+        subst; unfold fire in Hgt.
+        repeat compare_next; auto.
+        { get_enabled_constraints.
+          contradict Hgt.
+          omega.
+        }
+      }
+      { set (Hloop := even_odd_loop t' m m0 E O Hin).
+        destruct (IHm0 m0) as [IH1 [IH2 IH3]].
+        subst; unfold fire in Hgt.
+        repeat compare_next; auto.
+        { get_enabled_constraints.
+          contradict Hgt.
+          omega.
+        }
+      } 
+      { set (Hloop := even_odd_loop t' m m0 E O Hin).
+        destruct (IHm0 m0) as [IH1 [IH2 IH3]].
+        subst; unfold fire in Hgt.
+        repeat compare_next; auto.
+        { get_enabled_constraints.
+          contradict Hgt.
+          omega.
+        }
+      }
+    Qed.
+  End even_odd.
+
+  Section odd_even.
+    Variable O : odd.
+    Variable E : even.
+    Hypothesis Hin : In (O,E) (odd_even_neighbors c).
+    
+    Lemma odd_even_num_events : 
+       (m _ _ (Even_fall E) > 0 ->
+        num_events (Rise (Odd O)) t = num_events (Rise (Even E)) t)
+    /\ (m _ _ (Even_fall_odd_rise O E Hin) > 0 ->
+        num_events (Rise (Odd O)) t = num_events (Rise (Even E)) t)
+    /\ (m _ _ (Odd_rise_even_rise O E Hin) > 0 ->
+        num_events (Rise (Odd O)) t = 1 + num_events (Rise (Even E)) t).
+    Proof.
+      induction fd_t_m; repeat split; intros Hgt; simpl in *; auto; find_contradiction.
+      { set (Hloop := odd_even_loop t' m m0 O E Hin).
+        destruct (IHm0 m0) as [IH1 [IH2 IH3]].
+        subst; unfold fire in Hgt.
+        repeat compare_next; auto.
+        { get_enabled_constraints.
+          contradict Hgt.
+          omega.
+        }
+      }
+      { set (Hloop := odd_even_loop t' m m0 O E Hin).
+        destruct (IHm0 m0) as [IH1 [IH2 IH3]].
+        subst; unfold fire in Hgt.
+        repeat compare_next; auto.
+        { get_enabled_constraints.
+          contradict Hgt.
+          omega.
+        }
+      } 
+      { set (Hloop := odd_even_loop t' m m0 O E Hin).
+        destruct (IHm0 m0) as [IH1 [IH2 IH3]].
+        subst; unfold fire in Hgt.
+        repeat compare_next; auto.
+        { get_enabled_constraints.
+          contradict Hgt.
+          omega.
+        }
+      }
+    Qed.
+  End odd_even.
+    
+
+End fd_lemmas.
 
 
   Lemma fall_decoupled_strong : forall l t o v,
@@ -336,52 +505,46 @@ Admitted.
     * (* l is transparent *)
       rewrite H2.
 
-    (* n > 0 *)
-    destruct n as [|n].
-    { subst. destruct l as [O | E].
-        2:{ inversion Hn. }
-        (* since the initial state of odd latches are opaque *)
-        admit.
-    }
+      erewrite sync_eval_gt; eauto.
+      { (* n > 0 *)
+        subst.
+        destruct l as [O | E]; try omega.
 
-    erewrite sync_eval_S; auto.
+        erewrite odd_fall_num_events; eauto; try omega.
+        erewrite marking_odd_fall; eauto.
+        rewrite H. omega.
+      }
+
     intros l' Hl'. 
     erewrite H1; eauto.
     
-    inversion Hl'; subst.
-    { assert (Hfact : transparent P_FD t (Odd O) = Transparent ->
-                      num_events (Rise (Odd O)) t = 1+ num_events (Rise (Even E)) t)
-        by admit.
-      rewrite Hfact in Hn; auto.
-      inversion Hn.
-      reflexivity.
+    inversion Hl'; subst; f_equal.
+    { edestruct (even_odd_num_events t m Hm E O) as [HEO1 [HEO2 HEO3]]; eauto.
+      rewrite HEO1; auto.
+      erewrite marking_odd_fall; eauto.
+      rewrite H.
+      omega.
     }
-    { assert (Hfact : transparent P_FD t (Even E) = Transparent ->
-                      num_events (Rise (Even E)) t = num_events (Rise (Odd O)) t)
-        by admit.
-      inversion Hn.
-      rewrite Hfact; auto.
-    }
+    { edestruct (odd_even_num_events t m Hm O E) as [HOE1 [HOE2 HOE3]]; eauto.
+      rewrite HOE1; eauto; try omega.
+
+      erewrite marking_even_fall; eauto.
+      rewrite H; auto.
+   }
 
   * inversion Hm; subst.
     simpl in H. compare (Rise l) e.
     erewrite IHHrel; eauto.
     { destruct l; simpl; reduce_eqb; reflexivity. }
 
-  * 
-    destruct n as [|n].
-    { simpl in Hn. subst. destruct l as [O | E].
-        2:{ inversion Hn. }
-        (* since the initial state of odd latches are opaque *)
-        simpl in Hn.
-        rewrite sync_eval_odd_0.
-
-        inversion Hm; subst.
-        (* O- is enabled, but O+ has not yet occurred, this is a contradiction since O starts out low. *)
-        admit.
+  * inversion Hm.
+    assert (n > 0).
+    { subst. destruct l; try omega.
+      simpl.
+      erewrite odd_fall_num_events; eauto; try omega.
     }
 
-    erewrite sync_eval_S; eauto.
+    erewrite sync_eval_gt; eauto.
     intros l' Hl'.
 
     inversion Hm; subst.
@@ -390,426 +553,37 @@ Admitted.
     
     (* since Fall l is enabled *)
      inversion Hl'; subst.
-     { rewrite Hn.
-       f_equal. simpl.
-       assert (Hfact : transparent P_FD t (Odd O) = Transparent ->
-                      num_events (Rise (Odd O)) t = 1+ num_events (Rise (Even E)) t)
-        by admit.
-       rewrite Hfact; auto.
-       { (* since O- is enabled in t, O must be transparent in t *) admit. }
+     { f_equal. simpl.
+       get_enabled_constraints.
+       edestruct (even_odd_num_events) as [HEO1 [HEO2 HEO3]]; eauto.
+       erewrite HEO1; auto.
      }
-    { inversion Hn; subst.
-      assert (Hfact : transparent P_FD t (Even E) = Transparent ->
-                      num_events (Rise (Even E)) t = num_events (Rise (Odd O)) t)
-        by admit.
-      rewrite <- Hfact; auto.
-      { (* since E- is enabled in t, E must be transparent in t *) admit. }
-Admitted.
-
+    { f_equal. simpl. get_enabled_constraints. 
+      edestruct (odd_even_num_events t' m0 H8 O E) as [HOE1 [HOE2 HOE3]]; eauto.
+      erewrite HOE1; auto; try omega.
+    }
+    Unshelve. all:auto.
+Qed.
 
 
   Theorem fall_decoupled_flow_equivalence :
     flow_equivalence fall_decoupled c init_st P_FD.
   Proof.
-    intros l t v Heval [m Hm].
+    intros l t v [m Hm] Heval.
     erewrite (fall_decoupled_strong l t Opaque v Heval m Hm); eauto.
     
     destruct l as [O | E].
-    + erewrite num_events_odd_opaque; eauto.
-    + erewrite num_events_even_opaque; eauto.
+    + erewrite odd_rise_num_events; eauto.
+      erewrite marking_odd_rise; eauto.
+      erewrite async_b; eauto.
+      auto.
+    + erewrite even_rise_num_events; eauto.
+      erewrite marking_even_rise; eauto.
+      erewrite async_b; eauto.
+      auto.
   Qed.
     
 
-
-
-(*
-
-Lemma rise_enabled_even_odd : forall t m O E,
-    {fall_decoupled}⊢ t ↓ m ->
-    is_enabled fall_decoupled (Rise (Odd O)) m ->
-    In (E,O) (even_odd_neighbors c) ->
-    num_events (Rise (Even E)) t = num_events (Rise (Odd O)) t.
-Admitted.
-
-Lemma rise_enabled_odd_even : forall t m O E,
-    {fall_decoupled}⊢ t ↓ m ->
-    is_enabled fall_decoupled (Rise (Even E)) m ->
-    In (O,E) (odd_even_neighbors c) ->
-    num_events (Rise (Odd O)) t = 1+num_events (Rise (Even E)) t.
-Admitted.
-
-Lemma async_rel_transparent : forall l b t v,
-    async_rel c init_st l b t v ->
-    forall e,
-    e <> Rise l ->
-    e <> Fall l ->
-    transparent (next_trace e t) l = true ->
-    async_rel c init_st l true (next_trace e t) v.
-Proof.
-  intros l b t v Hrel.
-Import FE_Tactics.
-  induction Hrel; intros e0 Hrise Hfall Ht; reduce_transparent.
-  + econstructor; eauto.
-    { reduce_transparent. auto. }
-    intros l' [ | ] Hneighbor.
-    ++ (* true *)
-      compare e0 (Rise l').
-  Admitted.    
-*)
-
-
-(*
-
-Lemma event_fall_invariant_fd : forall l b t v,
-    async_rel c init_st l b t v ->
-    forall e,
-    e <> Rise l ->
-    forall m, {fall_decoupled}⊢ next_trace e t ↓ m ->
-    async_rel c init_st l (transparent (next_trace e t) l) (next_trace e t) v.
-Proof.
-    intros.
-    simpl. unfold fire_tstate.
-    reduce_eqb.
-    compare (Fall l) e.
-    { (* e = Fall l *)
-      econstructor; eauto.
-      simpl. unfold fire_tstate.
-      reduce_eqb. auto.
-    }
-
-    compare (transparent t l) false.
-    { rewrite e0. econstructor; eauto.
-      simpl. unfold fire_tstate.
-      reduce_eqb; auto.
-    }
-
-
-Qed.
-
-    *)
-
-
-
-Proof.
-  intros l e t v Hrel.
-Require Import Coq.Program.Equality.
-  remember (next_trace e t) as t'.
-  revert e t Heqt'.
-  induction Hrel as [? ? Hopaque | ? ? ? ? Htransparent ? | ? ? ? ? Hopaque ?];
-    intros e' t' Heqt' Hneq m Hm; subst.
-  * inversion Heqt'.
-  * inversion Hm; subst.
-    simpl in Htransparent.
-    unfold fire_tstate in Htransparent.
-    reduce_eqb.
-    compare (Fall l) e'.
-    eapply async_transparent; auto.
-    intros l' Hneighbor.
-    assert (transparent (next_trace e' t') l' = false).
-    { simpl. unfold fire_tstate.
-      (* since e' is enabled in m0 ~ t', if e' = Rise l', then l must have been
-      opaque, which is a contradiction. *)
-      (* if e' = Fall l', then we're good. *)
-      compare (Rise l') e'.
-      { contradict Htransparent. admit. }
-      compare (Fall l') e'; [auto | ].
-      admit (* induction? *).
-    }
-    
-
-    eapply H0; eauto.
-
-
-
-    apply Htransparent.
-
- as [? ? Hopaque | ? ? ? Htransparent ? | ? ? ? ? Hopaque Hrel]; intros e0 He0.
-  + 
-
-(*    
-Inductive sync_rel : nat -> latch even odd -> value -> Prop :=
-| Sync_odd_0 (O : odd) :  sync_rel 0 (Odd O) (init_st (Odd O)) (* Odd O ⇓^{0} init_st(Odd O)*)
-| Sync_odd_S (O : odd) (n : nat) (st0 : state (latch even odd)) :
-    (forall (E : even) (pf : In (E,O) (even_odd_neighbors c)), 
-            sync_rel (S n) (Even E) (st0(Even E))) ->
-    sync_rel (S n) (Odd O) (next_state c st0 (Odd O))
-| Sync_even_S (E : even) (n : nat) (st0 : state (latch even odd)) :
-    (forall (O : odd) (pf : In (O,E) (odd_even_neighbors c)), 
-            sync_rel n (Odd O) (st0(Odd O))) ->
-    sync_rel (S n) (Even E) (next_state c st0 (Even E))
-.
-
-Fixpoint length_trace (t : trace even odd) : nat :=
-  match t with
-  | empty_trace _ => 0
-  | next_trace _ t' => 1 + length_trace t'
-  end.
-*)
-
- Lemma event_fall_invariant_fd : forall n l v,
-    sync_rel n l v ->
-    forall t st st' e,
-    c ⊢ init_st ⇒t⇒ st ->
-    async_step c (transparent t) st e st' ->
-    e <> Rise l ->
-    transparent (next_trace e t) l = true ->
-    st'(l) = st(l).
-  Proof.
-    intros n l v Hrel.
-    induction Hrel; intros t st st' e Hst Hstep He Htransparent.
-    * simpl in Htransparent. unfold fire_tstate in *.
-      reduce_eqb.
-      compare (Fall (Odd O) : event even odd) e; [contradict Htransparent; auto | ].
-      destruct Hstep.
-      
-
-    * simpl in Htransparent. unfold fire_tstate in *.
-      reduce_eqb.
-      
-
-  Lemma event_disjoint_fd : forall n l v,
-    sync_rel n l v ->
-    forall t m st st',
-    {fall_decoupled}⊢ t ↓ m ->
-    n <= length_trace t ->
-    c ⊢ st ⇒t⇒st' ->
-    disjoint l t ->
-    transparent t l = true ->
-    st'(l) = st(l).
-  Proof.
-    intros n l v Hsync.
-    induction Hsync; intros t m st st' Hm Hlen Hst Hdisjoint Htransparent.
-    * contradict Htransparent. Search transparent Odd. admit (* true *).
-    * erewrite eval_transparent; eauto.
-      admit (* because O is disjoint from t and transaprent in t, it must also be transparent in the initial marking, which is a contradiction. *).
-    * erewrite eval_transparent; eauto.
-      transitivity (next_state c st (Even E)).
-      2:{ (* because E is disjoint from t and transaprent in t, it must also be transaprent in the initial marking. *) admit. }
-
-      simpl. apply f_equal. unfold odd_state.
-      apply functional_extensionality. intros [O Hpf]. simpl.
-
-      assert (
-
-
-    {fall_decoupled}⊢ t ↓ m ->
-    c ⊢ st ⇒t⇒ st' ->
-    disjoint l t ->
-    st'(l) = st(l).
-  Proof.
-    intros t m st st' l Hm Hst Hdisjoint.
-    revert m st st' Hm Hst.
-    induction Hdisjoint; intros m st st' Hm Hst.
-    *  inversion Hst; auto.
-    * 
-
-    induction t as [P | e t]; intros m st st' l Hm Hst Hdisjoint.
-    * inversion Hst. reflexivity.
-    * inversion Hst as [ | e0 t0  st0 st'0 Hst' Hopaque Htransparent]; subst.
-      inversion Hdisjoint as [ | l0 e0 t0 e_neq_l Hpred Hdisjoint']; subst.
-      inversion Hm as [ | e0 m' m0' t0 Henabled Hfire Hm']; subst.
-      
-
-  Admitted.
-
-  Lemma event_fall_invariant_fd : forall t st l st',
-    c ⊢ init_st ⇒t⇒ st ->
-    async_step c (transparent t) st (Fall l) st' ->
-    forall l', st'(l') = st(l').
-  Proof.
-(*
-    induction t as [P | e t]; intros st l st' Hst [Hopaque Htransparent] l'.
-    * (* t = [] *)
-      inversion Hst as [P0 Htransparencies | ]; subst.
-     
-
-    destruct ((fire_tstate (Fall l) P) l')
-      eqn:Hl';
-      unfold fire_tstate in Hl';
-      simpl in Hl'.
-    + (* l is transparent *)
-      compare l l'; [contradict Hl'; auto | ].
-      rewrite eqb_neq in Hl'; [ | inversion 1; subst; contradiction].
-      
-     
-
-    destruct ((fire_tstate (Fall l) (transparent t)) l')
-      eqn:Hl'.
-    * (* l' is transparent *)
-
-      rewrite Htransparent; auto.
-
-      unfold fire_tstate in Hl'.
-      simpl in Hl'.
-      assert (Fall l' <> Fall l).
-      { inversion 1; subst. rewrite eqb_eq in Hl'. inversion Hl'. }
-      rewrite eqb_neq in Hl'; auto.
-
-      erewrite (eval_transparent _ _ t st); eauto.
-      unfold next_state.
-
-      admit (* need induction? *).
-    * (* l' is opaque *)
-      unfold fire_tstate in Hl'.
-      simpl in Hl'.
-Existing Instance latch_eq_dec.
-      destruct (Dec l' l).
-      ** subst.
-         erewrite Hopaque; eauto.
-      ** rewrite eqb_neq in Hl'; [ | inversion 1; contradiction].
-         rewrite Hopaque; auto.
-         unfold fire_tstate. simpl.
-         rewrite eqb_neq; auto.
-         inversion 1; contradiction.
-*)
-  Admitted.
-
-
-  Lemma event_rise_invariant_fd : forall t m st st' l,
-    {fall_decoupled}⊢ t ↓ m ->
-    c ⊢ init_st ⇒t⇒ st ->
-    async_step c (transparent t) st (Rise l) st' ->
-    forall l', l' <> l -> st'(l') = st(l').
-  Admitted.
-
-  Lemma event_invariant_neq : forall t m st st' e,
-    {fall_decoupled}⊢ t ↓ m ->
-    c ⊢ init_st ⇒t⇒ st ->
-    async_step c (transparent t) st e st' ->
-    forall l, e <> Rise l -> st'(l) = st(l).
-  Proof.
-    intros t m st st' e Hm Hst Hstep l Hl.
-    destruct e as [l' | l'].
-    * eapply event_rise_invariant_fd; eauto.
-      inversion 1; subst; contradiction.
-    * eapply event_fall_invariant_fd; eauto.
-  Qed.
-
-
-
-
-Opaque sync_eval.
-  Lemma fall_decoupled_strong : 
-    forall t,
-      forall m, {fall_decoupled}⊢ t ↓ m ->
-      forall st, c ⊢ init_st ⇒t⇒ st ->
-      (forall O, st(Odd O) = sync_eval c init_st (num_events (Rise (Odd O)) t) (Odd O)) /\
-      (forall E, st(Even E) = sync_eval c init_st (1+num_events (Rise (Even E)) t) (Even E)).
-  Proof.
-    induction t as [P | e t];
-      intros m Hm st Heval;
-      split; intros l.
-    * (* base case, odd *)
-      simpl. inversion Heval; subst. reflexivity.
-    * (* base case, even *)
-      simpl. inversion Heval; subst.
-      erewrite eval_transparent; eauto.
-      { simpl. rewrite sync_eval_even. reflexivity.
-      }
-      { simpl.
-        inversion Hm as [P0 Hopaque Htransparent | ]; clear H P0; rewrite <- H2 in *; clear m H2.
-        apply Htransparent.
-
-        apply FD_is_enabled_equiv.
-        constructor; auto.
-      }
-    * (* inductive case, odd *)
-
-      inversion Hm as [ | e0' m0 m0' s' Henabled Hfire Hconsistent']; subst;
-        rename m0 into m.
-      inversion Heval as [ | ? ? st' ? Heval' Hopaque' Htransparent']; subst.
-      simpl in *.
-
-      destruct (Dec (Rise (Odd l)) e).
-      (* If e = l+, then l is transparent in (e::t) *)
-      { subst. rewrite eqb_eq.
-        rewrite Htransparent'.
-        2:{ unfold fire_tstate. rewrite eqb_eq. auto. }
-        simpl.
-        rewrite sync_eval_odd.
-        
-        f_equal. apply functional_extensionality. 
-        unfold even_state. intros [E He].
-        simpl.
-
-        rewrite (event_rise_invariant_fd t m st' st (Odd l)); auto.
-        2:{ split; auto. }
-        2:{ inversion 1. }
-
-        destruct (IHt m Hconsistent' st' Heval') as [_ IH].
-        rewrite IH.
-        
-        assert (Hnum : num_events (Rise (Even E)) t = num_events (Rise (Odd l)) t).
-        { eapply rise_enabled_even_odd; eauto.  }
-
-        rewrite Hnum. reflexivity.
-      }
-
-      rewrite eqb_neq; auto.
-    
-      rewrite (event_invariant_neq t m st' st e); eauto.
-      2:{ split; auto. }
-
-      destruct (IHt m Hconsistent' st' Heval') as [IH _].
-      rewrite IH.
-      reflexivity.
-      
-      
-
-    * (* inductive case, even *)
-      inversion Hm as [ | e0' m0 m0' s' Henabled Hfire Hconsistent']; subst;
-        rename m0 into m.
-      inversion Heval as [ | ? ? st' ? Heval' Hopaque' Htransparent']; subst.
-      simpl in *.
-
-      destruct (Dec (Rise (Even l)) e).
-      (* If e = l+, then l is transparent in (e::t) *)
-      { subst. rewrite eqb_eq.
-        rewrite Htransparent'.
-        2:{ unfold fire_tstate. rewrite eqb_eq. auto. }
-        simpl.
-        rewrite sync_eval_even.
-        
-        f_equal. apply functional_extensionality. 
-        unfold odd_state. intros [O He].
-        simpl.
-
-        rewrite (event_rise_invariant_fd t m st' st (Even l)); auto.
-        2:{ split; auto. }
-        2:{ inversion 1. }
-
-        destruct (IHt m Hconsistent' st' Heval') as [IH _].
-        rewrite IH.
-        
-        assert (Hnum : num_events (Rise (Odd O)) t = 1+num_events (Rise (Even l)) t).
-        { eapply rise_enabled_odd_even; eauto. }
-
-        rewrite Hnum. reflexivity.
-      }
-
-      rewrite eqb_neq; auto.
-    
-      rewrite (event_invariant_neq t m st' st e); eauto.
-      2:{ split; auto. }
-      destruct (IHt m Hconsistent' st' Heval') as [_ IH].
-      rewrite IH.
-      reflexivity.
-  Qed.
-      
-
-
-        
-  Theorem fall_decoupled_flow_equivalence :
-    flow_equivalence fall_decoupled c init_st.
-  Proof.
-    intros t [m Hm] st Hst l Hopaque.
-    destruct (fall_decoupled_strong t m Hm st Hst) as [HO HE].
-    destruct l as [O | E].
-    + rewrite HO.
-      erewrite num_events_odd_opaque; eauto.
-    + rewrite HE.
-      erewrite num_events_even_opaque; eauto.
-  Qed.
 
 
 End FallDecoupled.
